arm/proofs/sha3_keccak2_f1600_alt.ml
@@ -10,11 +10,11 @@
 needs "arm/proofs/base.ml";;
 needs "arm/proofs/utils/keccak_spec.ml";;
 
-(**** print_literal_from_elf "arm/mlkem/mlkem_keccak2_f1600.o";;
+(**** print_literal_from_elf "arm/sha3/sha3_keccak2_f1600_alt.o";;
  ****)
 
-let mlkem_keccak2_f1600_mc = define_assert_from_elf
-  "mlkem_keccak2_f1600_mc" "arm/mlkem/mlkem_keccak2_f1600.o"
+let sha3_keccak2_f1600_alt_mc = define_assert_from_elf
+  "sha3_keccak2_f1600_alt_mc" "arm/sha3/sha3_keccak2_f1600_alt.o"
 [
   0xd10103ff;       (* arm_SUB SP SP (rvalue (word 64)) *)
   0x6d0027e8;       (* arm_STP D8 D9 SP (Immediate_Offset (iword (&0))) *)
@@ -62,75 +62,122 @@ let mlkem_keccak2_f1600_mc = define_assert_from_elf
   0xfd406059;       (* arm_LDR D25 X2 (Immediate_Offset (word 192)) *)
   0x4ed92b18;       (* arm_TRN1 Q24 Q24 Q25 64 128 *)
   0xd2800302;       (* arm_MOV X2 (rvalue (word 24)) *)
-  0xce05281e;       (* arm_EOR3 Q30 Q0 Q5 Q10 *)
-  0xce062c3d;       (* arm_EOR3 Q29 Q1 Q6 Q11 *)
-  0xce07305c;       (* arm_EOR3 Q28 Q2 Q7 Q12 *)
-  0xce08347b;       (* arm_EOR3 Q27 Q3 Q8 Q13 *)
-  0xce09389a;       (* arm_EOR3 Q26 Q4 Q9 Q14 *)
+  0x6e251c1e;       (* arm_EOR_VEC Q30 Q0 Q5 128 *)
+  0x6e2a1fde;       (* arm_EOR_VEC Q30 Q30 Q10 128 *)
   0xce0f53de;       (* arm_EOR3 Q30 Q30 Q15 Q20 *)
+  0x6e261c3d;       (* arm_EOR_VEC Q29 Q1 Q6 128 *)
+  0x6e2b1fbd;       (* arm_EOR_VEC Q29 Q29 Q11 128 *)
   0xce1057bd;       (* arm_EOR3 Q29 Q29 Q16 Q21 *)
+  0x6e271c5c;       (* arm_EOR_VEC Q28 Q2 Q7 128 *)
+  0x6e2c1f9c;       (* arm_EOR_VEC Q28 Q28 Q12 128 *)
   0xce115b9c;       (* arm_EOR3 Q28 Q28 Q17 Q22 *)
+  0x6e281c7b;       (* arm_EOR_VEC Q27 Q3 Q8 128 *)
+  0x6e2d1f7b;       (* arm_EOR_VEC Q27 Q27 Q13 128 *)
   0xce125f7b;       (* arm_EOR3 Q27 Q27 Q18 Q23 *)
+  0x6e291c9a;       (* arm_EOR_VEC Q26 Q4 Q9 128 *)
+  0x6e2e1f5a;       (* arm_EOR_VEC Q26 Q26 Q14 128 *)
   0xce13635a;       (* arm_EOR3 Q26 Q26 Q19 Q24 *)
-  0xce7c8fd9;       (* arm_RAX1 Q25 Q30 Q28 *)
+  0x4efc879f;       (* arm_ADD_VEC Q31 Q28 Q28 64 128 *)
+  0x6f41479f;       (* arm_SRI_VEC Q31 Q28 63 64 128 *)
+  0x6e3e1ff9;       (* arm_EOR_VEC Q25 Q31 Q30 128 *)
   0xce7a8f9c;       (* arm_RAX1 Q28 Q28 Q26 *)
-  0xce7d8f5a;       (* arm_RAX1 Q26 Q26 Q29 *)
+  0x4efd87bf;       (* arm_ADD_VEC Q31 Q29 Q29 64 128 *)
+  0x6f4147bf;       (* arm_SRI_VEC Q31 Q29 63 64 128 *)
+  0x6e3a1ffa;       (* arm_EOR_VEC Q26 Q31 Q26 128 *)
   0xce7b8fbd;       (* arm_RAX1 Q29 Q29 Q27 *)
-  0xce7e8f7b;       (* arm_RAX1 Q27 Q27 Q30 *)
+  0x4efe87df;       (* arm_ADD_VEC Q31 Q30 Q30 64 128 *)
+  0x6f4147df;       (* arm_SRI_VEC Q31 Q30 63 64 128 *)
+  0x6e3b1ffb;       (* arm_EOR_VEC Q27 Q31 Q27 128 *)
   0x6e3a1c1e;       (* arm_EOR_VEC Q30 Q0 Q26 128 *)
   0xce9d0840;       (* arm_XAR Q0 Q2 Q29 (word 2) *)
-  0xce9d5582;       (* arm_XAR Q2 Q12 Q29 (word 21) *)
+  0x6e3d1d9f;       (* arm_EOR_VEC Q31 Q12 Q29 128 *)
+  0x4f6b57e2;       (* arm_SHL_VEC Q2 Q31 43 64 128 *)
+  0x6f6b47e2;       (* arm_SRI_VEC Q2 Q31 21 64 128 *)
   0xce9c9dac;       (* arm_XAR Q12 Q13 Q28 (word 39) *)
-  0xce9be26d;       (* arm_XAR Q13 Q19 Q27 (word 56) *)
+  0x6e3b1e7f;       (* arm_EOR_VEC Q31 Q19 Q27 128 *)
+  0x4f4857ed;       (* arm_SHL_VEC Q13 Q31 8 64 128 *)
+  0x6f4847ed;       (* arm_SRI_VEC Q13 Q31 56 64 128 *)
   0xce9c22f3;       (* arm_XAR Q19 Q23 Q28 (word 8) *)
-  0xce9a5df7;       (* arm_XAR Q23 Q15 Q26 (word 23) *)
+  0x6e3a1dff;       (* arm_EOR_VEC Q31 Q15 Q26 128 *)
+  0x4f6957f7;       (* arm_SHL_VEC Q23 Q31 41 64 128 *)
+  0x6f6947f7;       (* arm_SRI_VEC Q23 Q31 23 64 128 *)
   0xce99fc2f;       (* arm_XAR Q15 Q1 Q25 (word 63) *)
-  0xce9c2501;       (* arm_XAR Q1 Q8 Q28 (word 9) *)
+  0x6e3c1d1f;       (* arm_EOR_VEC Q31 Q8 Q28 128 *)
+  0x4f7757e1;       (* arm_SHL_VEC Q1 Q31 55 64 128 *)
+  0x6f7747e1;       (* arm_SRI_VEC Q1 Q31 9 64 128 *)
   0xce994e08;       (* arm_XAR Q8 Q16 Q25 (word 19) *)
-  0xce9de8f0;       (* arm_XAR Q16 Q7 Q29 (word 58) *)
+  0x6e3d1cff;       (* arm_EOR_VEC Q31 Q7 Q29 128 *)
+  0x4f4657f0;       (* arm_SHL_VEC Q16 Q31 6 64 128 *)
+  0x6f4647f0;       (* arm_SRI_VEC Q16 Q31 58 64 128 *)
   0xce9af547;       (* arm_XAR Q7 Q10 Q26 (word 61) *)
-  0xce9c906a;       (* arm_XAR Q10 Q3 Q28 (word 36) *)
+  0x6e3c1c7f;       (* arm_EOR_VEC Q31 Q3 Q28 128 *)
+  0x4f5c57ea;       (* arm_SHL_VEC Q10 Q31 28 64 128 *)
+  0x6f5c47ea;       (* arm_SRI_VEC Q10 Q31 36 64 128 *)
   0xce9cae43;       (* arm_XAR Q3 Q18 Q28 (word 43) *)
-  0xce9dc632;       (* arm_XAR Q18 Q17 Q29 (word 49) *)
+  0x6e3d1e3f;       (* arm_EOR_VEC Q31 Q17 Q29 128 *)
+  0x4f4f57f2;       (* arm_SHL_VEC Q18 Q31 15 64 128 *)
+  0x6f4f47f2;       (* arm_SRI_VEC Q18 Q31 49 64 128 *)
   0xce99d971;       (* arm_XAR Q17 Q11 Q25 (word 54) *)
-  0xce9bb12b;       (* arm_XAR Q11 Q9 Q27 (word 44) *)
+  0x6e3b1d3f;       (* arm_EOR_VEC Q31 Q9 Q27 128 *)
+  0x4f5457eb;       (* arm_SHL_VEC Q11 Q31 20 64 128 *)
+  0x6f5447eb;       (* arm_SRI_VEC Q11 Q31 44 64 128 *)
   0xce9d0ec9;       (* arm_XAR Q9 Q22 Q29 (word 3) *)
-  0xce9b65d6;       (* arm_XAR Q22 Q14 Q27 (word 25) *)
+  0x6e3b1ddf;       (* arm_EOR_VEC Q31 Q14 Q27 128 *)
+  0x4f6757f6;       (* arm_SHL_VEC Q22 Q31 39 64 128 *)
+  0x6f6747f6;       (* arm_SRI_VEC Q22 Q31 25 64 128 *)
   0xce9aba8e;       (* arm_XAR Q14 Q20 Q26 (word 46) *)
-  0xce9b9494;       (* arm_XAR Q20 Q4 Q27 (word 37) *)
+  0x6e3b1c9f;       (* arm_EOR_VEC Q31 Q4 Q27 128 *)
+  0x4f5b57f4;       (* arm_SHL_VEC Q20 Q31 27 64 128 *)
+  0x6f5b47f4;       (* arm_SRI_VEC Q20 Q31 37 64 128 *)
   0xce9bcb04;       (* arm_XAR Q4 Q24 Q27 (word 50) *)
-  0xce99fab8;       (* arm_XAR Q24 Q21 Q25 (word 62) *)
+  0x6e391ebf;       (* arm_EOR_VEC Q31 Q21 Q25 128 *)
+  0x4f4257f8;       (* arm_SHL_VEC Q24 Q31 2 64 128 *)
+  0x6f4247f8;       (* arm_SRI_VEC Q24 Q31 62 64 128 *)
   0xce9a70b5;       (* arm_XAR Q21 Q5 Q26 (word 28) *)
-  0xce9950db;       (* arm_XAR Q27 Q6 Q25 (word 20) *)
-  0x4ddfcc3f;       (* arm_LD1R Q31 X1 (Postimmediate_Offset (word 8)) 64 128 *)
+  0x6e391cdf;       (* arm_EOR_VEC Q31 Q6 Q25 128 *)
+  0x4f6c57fb;       (* arm_SHL_VEC Q27 Q31 44 64 128 *)
+  0x6f6c47fb;       (* arm_SRI_VEC Q27 Q31 20 64 128 *)
+  0x4ddfcc3c;       (* arm_LD1R Q28 X1 (Postimmediate_Offset (word 8)) 64 128 *)
   0xce272d45;       (* arm_BCAX Q5 Q10 Q7 Q11 *)
-  0xce281d66;       (* arm_BCAX Q6 Q11 Q8 Q7 *)
+  0x4e671d1f;       (* arm_BIC_VEC Q31 Q8 Q7 128 *)
+  0x6e2b1fe6;       (* arm_EOR_VEC Q6 Q31 Q11 128 *)
   0xce2920e7;       (* arm_BCAX Q7 Q7 Q9 Q8 *)
-  0xce2a2508;       (* arm_BCAX Q8 Q8 Q10 Q9 *)
+  0x4e691d5f;       (* arm_BIC_VEC Q31 Q10 Q9 128 *)
+  0x6e281fe8;       (* arm_EOR_VEC Q8 Q31 Q8 128 *)
   0xce2b2929;       (* arm_BCAX Q9 Q9 Q11 Q10 *)
-  0xce2c41ea;       (* arm_BCAX Q10 Q15 Q12 Q16 *)
+  0x4e701d9f;       (* arm_BIC_VEC Q31 Q12 Q16 128 *)
+  0x6e2f1fea;       (* arm_EOR_VEC Q10 Q31 Q15 128 *)
   0xce2d320b;       (* arm_BCAX Q11 Q16 Q13 Q12 *)
-  0xce2e358c;       (* arm_BCAX Q12 Q12 Q14 Q13 *)
+  0x4e6d1ddf;       (* arm_BIC_VEC Q31 Q14 Q13 128 *)
+  0x6e2c1fec;       (* arm_EOR_VEC Q12 Q31 Q12 128 *)
   0xce2f39ad;       (* arm_BCAX Q13 Q13 Q15 Q14 *)
-  0xce303dce;       (* arm_BCAX Q14 Q14 Q16 Q15 *)
+  0x4e6f1e1f;       (* arm_BIC_VEC Q31 Q16 Q15 128 *)
+  0x6e2e1fee;       (* arm_EOR_VEC Q14 Q31 Q14 128 *)
   0xce31568f;       (* arm_BCAX Q15 Q20 Q17 Q21 *)
-  0xce3246b0;       (* arm_BCAX Q16 Q21 Q18 Q17 *)
+  0x4e711e5f;       (* arm_BIC_VEC Q31 Q18 Q17 128 *)
+  0x6e351ff0;       (* arm_EOR_VEC Q16 Q31 Q21 128 *)
   0xce334a31;       (* arm_BCAX Q17 Q17 Q19 Q18 *)
-  0xce344e52;       (* arm_BCAX Q18 Q18 Q20 Q19 *)
+  0x4e731e9f;       (* arm_BIC_VEC Q31 Q20 Q19 128 *)
+  0x6e321ff2;       (* arm_EOR_VEC Q18 Q31 Q18 128 *)
   0xce355273;       (* arm_BCAX Q19 Q19 Q21 Q20 *)
-  0xce360414;       (* arm_BCAX Q20 Q0 Q22 Q1 *)
+  0x4e611edf;       (* arm_BIC_VEC Q31 Q22 Q1 128 *)
+  0x6e201ff4;       (* arm_EOR_VEC Q20 Q31 Q0 128 *)
   0xce375835;       (* arm_BCAX Q21 Q1 Q23 Q22 *)
-  0xce385ed6;       (* arm_BCAX Q22 Q22 Q24 Q23 *)
+  0x4e771f1f;       (* arm_BIC_VEC Q31 Q24 Q23 128 *)
+  0x6e361ff6;       (* arm_EOR_VEC Q22 Q31 Q22 128 *)
   0xce2062f7;       (* arm_BCAX Q23 Q23 Q0 Q24 *)
-  0xce210318;       (* arm_BCAX Q24 Q24 Q1 Q0 *)
+  0x4e601c3f;       (* arm_BIC_VEC Q31 Q1 Q0 128 *)
+  0x6e381ff8;       (* arm_EOR_VEC Q24 Q31 Q24 128 *)
   0xce226fc0;       (* arm_BCAX Q0 Q30 Q2 Q27 *)
-  0xce230b61;       (* arm_BCAX Q1 Q27 Q3 Q2 *)
+  0x4e621c7f;       (* arm_BIC_VEC Q31 Q3 Q2 128 *)
+  0x6e3b1fe1;       (* arm_EOR_VEC Q1 Q31 Q27 128 *)
   0xce240c42;       (* arm_BCAX Q2 Q2 Q4 Q3 *)
-  0xce3e1063;       (* arm_BCAX Q3 Q3 Q30 Q4 *)
+  0x4e641fdf;       (* arm_BIC_VEC Q31 Q30 Q4 128 *)
+  0x6e231fe3;       (* arm_EOR_VEC Q3 Q31 Q3 128 *)
   0xce3b7884;       (* arm_BCAX Q4 Q4 Q27 Q30 *)
-  0x6e3f1c00;       (* arm_EOR_VEC Q0 Q0 Q31 128 *)
+  0x6e3c1c00;       (* arm_EOR_VEC Q0 Q0 Q28 128 *)
   0xd1000442;       (* arm_SUB X2 X2 (rvalue (word 1)) *)
-  0xb5fff782;       (* arm_CBNZ X2 (word 2096880) *)
+  0xb5fff1a2;       (* arm_CBNZ X2 (word 2096692) *)
   0x91032002;       (* arm_ADD X2 X0 (rvalue (word 200)) *)
   0x4ec12819;       (* arm_TRN1 Q25 Q0 Q1 64 128 *)
   0x4ec3285a;       (* arm_TRN1 Q26 Q2 Q3 64 128 *)
@@ -179,23 +226,23 @@ let mlkem_keccak2_f1600_mc = define_assert_from_elf
   0xd65f03c0        (* arm_RET X30 *)
 ];;
 
-let MLKEM_KECCAK2_F1600_EXEC = ARM_MK_EXEC_RULE mlkem_keccak2_f1600_mc;;
+let SHA3_KECCAK2_F1600_ALT_EXEC = ARM_MK_EXEC_RULE sha3_keccak2_f1600_alt_mc;;
 
 (* ------------------------------------------------------------------------- *)
 (* Correctness proof                                                         *)
 (* ------------------------------------------------------------------------- *)
 
-let MLKEM_KECCAK2_F1600_CORRECT = prove
+let SHA3_KECCAK2_F1600_ALT_CORRECT = prove
  (`!a rc A A' pc.
-      ALL (nonoverlapping (a,400)) [(word pc,0x284); (rc,192)]
+      ALL (nonoverlapping (a,400)) [(word pc,0x340); (rc,192)]
       ==> ensures arm
-           (\s. aligned_bytes_loaded s (word pc) mlkem_keccak2_f1600_mc /\
+           (\s. aligned_bytes_loaded s (word pc) sha3_keccak2_f1600_alt_mc /\
                 read PC s = word (pc + 0x14) /\
                 C_ARGUMENTS [a; rc] s /\
                 wordlist_from_memory(a,25) s = A /\
                 wordlist_from_memory(word_add a (word 200),25) s = A' /\
                 wordlist_from_memory(rc,24) s = round_constants)
-           (\s. read PC s = word(pc + 0x26c) /\
+           (\s. read PC s = word(pc + 0x328) /\
                 wordlist_from_memory(a,25) s = keccak 24 A /\
                 wordlist_from_memory(word_add a (word 200),25) s = keccak 24 A')
            (MAYCHANGE_REGS_AND_FLAGS_PERMITTED_BY_ABI ,,
@@ -203,7 +250,7 @@ let MLKEM_KECCAK2_F1600_CORRECT = prove
             MAYCHANGE [memory :> bytes(a,400)])`,
   MAP_EVERY X_GEN_TAC
    [`a:int64`; `rc:int64`; `A:int64 list`; `A':int64 list`; `pc:num`] THEN
-  REWRITE_TAC[fst MLKEM_KECCAK2_F1600_EXEC] THEN
+  REWRITE_TAC[fst SHA3_KECCAK2_F1600_ALT_EXEC] THEN
   REWRITE_TAC[MAYCHANGE_REGS_AND_FLAGS_PERMITTED_BY_ABI; C_ARGUMENTS;
               ALL; ALLPAIRS; NONOVERLAPPING_CLAUSES] THEN
   DISCH_THEN(REPEAT_TCL CONJUNCTS_THEN ASSUME_TAC) THEN
@@ -219,7 +266,7 @@ let MLKEM_KECCAK2_F1600_CORRECT = prove
     CONV_TAC(ONCE_DEPTH_CONV WORDLIST_FROM_MEMORY_CONV) THEN
     REWRITE_TAC[LENGTH; ARITH] THEN ASM_MESON_TAC[]] THEN
 
-  ENSURES_WHILE_UP_TAC `24` `pc + 0xb8` `pc + 0x1c8`
+  ENSURES_WHILE_UP_TAC `24` `pc + 0xb8` `pc + 0x284`
    `\i s.
       wordlist_from_memory(rc,24) s = round_constants /\
       read X0 s = a /\
@@ -248,7 +295,7 @@ let MLKEM_KECCAK2_F1600_CORRECT = prove
     MEMORY_128_FROM_64_TAC "a" 0 12 THEN
     MEMORY_128_FROM_64_TAC "a" 200 12 THEN
     ASM_REWRITE_TAC[WORD_ADD_0] THEN STRIP_TAC THEN STRIP_TAC THEN
-    ARM_STEPS_TAC MLKEM_KECCAK2_F1600_EXEC (1--41) THEN
+    ARM_STEPS_TAC SHA3_KECCAK2_F1600_ALT_EXEC (1--41) THEN
     ENSURES_FINAL_STATE_TAC THEN ASM_REWRITE_TAC[] THEN
     REPLICATE_TAC 2 (CONJ_TAC THENL [CONV_TAC WORD_RULE; ALL_TAC]) THEN
     MAP_EVERY EXPAND_TAC ["A"; "A'"] THEN
@@ -275,19 +322,19 @@ let MLKEM_KECCAK2_F1600_CORRECT = prove
       ASM_REWRITE_TAC[round_constants; WORD_ADD_0] THEN
       CONV_TAC(ONCE_DEPTH_CONV EL_CONV) THEN REWRITE_TAC[];
       ALL_TAC] THEN
-    ARM_STEPS_TAC MLKEM_KECCAK2_F1600_EXEC (1--68) THEN
+    ARM_STEPS_TAC SHA3_KECCAK2_F1600_ALT_EXEC (1--115) THEN
     ENSURES_FINAL_STATE_TAC THEN ASM_REWRITE_TAC[] THEN
     REPEAT(CONJ_TAC THENL [CONV_TAC WORD_RULE; ALL_TAC]) THEN
     REWRITE_TAC[keccak; keccak_round] THEN
     CONV_TAC(TOP_DEPTH_CONV let_CONV) THEN REWRITE_TAC[MAP2; CONS_11] THEN
-    REPEAT CONJ_TAC THEN BITBLAST_TAC;
+    POP_ASSUM_LIST(K ALL_TAC) THEN REPEAT CONJ_TAC THEN BITBLAST_TAC;
 
     (*** The trivial loop-back goal ***)
 
     X_GEN_TAC `i:num` THEN STRIP_TAC THEN
     REWRITE_TAC[round_constants; CONS_11; GSYM CONJ_ASSOC;
      WORDLIST_FROM_MEMORY_CONV `wordlist_from_memory(rc,24) s:int64 list`] THEN
-    ARM_SIM_TAC MLKEM_KECCAK2_F1600_EXEC [1] THEN
+    ARM_SIM_TAC SHA3_KECCAK2_F1600_ALT_EXEC [1] THEN
     VAL_INT64_TAC `i:num` THEN
     ASM_REWRITE_TAC[] THEN CONV_TAC(DEPTH_CONV WORD_NUM_RED_CONV) THEN
     ASM_SIMP_TAC[LT_IMP_NE];
@@ -300,7 +347,7 @@ let MLKEM_KECCAK2_F1600_CORRECT = prove
     DISCH_THEN(CONJUNCTS_THEN SUBST1_TAC) THEN
     REWRITE_TAC[MAP2; CONS_11; GSYM CONJ_ASSOC] THEN
 
-    ARM_SIM_TAC MLKEM_KECCAK2_F1600_EXEC (1--41) THEN
+    ARM_SIM_TAC SHA3_KECCAK2_F1600_ALT_EXEC (1--41) THEN
     CONV_TAC(ONCE_DEPTH_CONV WORDLIST_FROM_MEMORY_CONV) THEN
 
     REPEAT(FIRST_X_ASSUM(STRIP_ASSUME_TAC o
@@ -310,15 +357,15 @@ let MLKEM_KECCAK2_F1600_CORRECT = prove
     ASM_REWRITE_TAC[] THEN
     REWRITE_TAC[CONS_11] THEN REPEAT CONJ_TAC THEN CONV_TAC WORD_BLAST]);;
 
-let MLKEM_KECCAK2_F1600_SUBROUTINE_CORRECT = prove
+let SHA3_KECCAK2_F1600_ALT_SUBROUTINE_CORRECT = prove
 (`!a rc A A' pc stackpointer returnaddress.
         aligned 16 stackpointer /\
         nonoverlapping (a,400) (word_sub stackpointer (word 64),64) /\
         ALLPAIRS nonoverlapping
           [(a,400); (word_sub stackpointer (word 64),64)]
-          [(word pc,0x284); (rc,192)]
+          [(word pc,0x340); (rc,192)]
         ==> ensures arm
-             (\s. aligned_bytes_loaded s (word pc) mlkem_keccak2_f1600_mc /\
+             (\s. aligned_bytes_loaded s (word pc) sha3_keccak2_f1600_alt_mc /\
                   read PC s = word pc /\
                   read SP s = stackpointer /\
                   read X30 s = returnaddress /\
@@ -338,6 +385,6 @@ let MLKEM_KECCAK2_F1600_SUBROUTINE_CORRECT = prove
     (WORDLIST_FROM_MEMORY_CONV THENC
      ONCE_DEPTH_CONV NORMALIZE_RELATIVE_ADDRESS_CONV) in
   CONV_TAC TWEAK_CONV THEN
-  ARM_ADD_RETURN_STACK_TAC ~pre_post_nsteps:(5,5) MLKEM_KECCAK2_F1600_EXEC
-   (CONV_RULE TWEAK_CONV MLKEM_KECCAK2_F1600_CORRECT)
+  ARM_ADD_RETURN_STACK_TAC ~pre_post_nsteps:(5,5) SHA3_KECCAK2_F1600_ALT_EXEC
+   (CONV_RULE TWEAK_CONV SHA3_KECCAK2_F1600_ALT_CORRECT)
   `[D8; D9; D10; D11; D12; D13; D14; D15]` 64);;
